arch_split x64 arm: make endpoint_bits and ntfn_bits arch constants

spec/abstract/ARM/Arch_Structs_A.thy
@@ -127,6 +127,12 @@ where
 | "arch_cap_is_device (PageTableCap x as3) = False"
 | "arch_cap_is_device (PageDirectoryCap x as2) = False"
 
+definition endpoint_bits :: nat where
+  "endpoint_bits \<equiv> 4"
+
+definition ntfn_bits :: nat where
+  "ntfn_bits \<equiv> 4"
+
 primrec
   arch_kobj_size :: "arch_kernel_obj \<Rightarrow> nat"
 where
